Mutable works

prototype/unstacked_borrows_pseudo.dfy
@@ -26,8 +26,8 @@ class State {
    predicate valid()
    reads this, mem, tagmem, rawfrom;
    {
-    mem.Length == tagmem.Length && mem.Length == rawfrom.Length &&
-    forall i:: 0 <= i && i < tagmem.Length && tagmem[i].Unique? ==> tagmem[i].t <= counter
+    mem.Length == tagmem.Length && mem.Length == rawfrom.Length 
+    && forall i:: 0 <= i && i < tagmem.Length && tagmem[i].Unique? ==> tagmem[i].t <= counter
    } 
 
    predicate valid_addr(addr: int)
@@ -44,7 +44,7 @@ predicate invalidTag(addr: nat, tag: Tag, predecessor: Tag)
     match (tagmem[addr], tag, predecessor)
     case (Unique(n1, c1), Unique(n2, c2),  Unique(n3, c3)) => 
      if (rawfrom[addr] != -1) then n2 != n1
-      else n1 < n2 || (n1 > n2 && n3 <= n1)  // C2 || C1
+      else n1 < n2 || (n1 > n2 && n3 <= n1)
     case (SharedRO(n1, c1), Unique(n2, c2), _) => 
      if (rawfrom[addr] != -1) then true 
      else false  // unknown
@@ -78,17 +78,6 @@ reads this, tagmem, rawfrom, mem;
      counter := counter + 1;
      ret := counter;
    }
-
-   predicate valid_predecessor(tag: Tag, predec: Tag)
-   reads this;
-   {
-     match (tag, predec)
-       case (Unique(n1, c1), Unique(n2, c2)) =>  n2 < n1
-       case (SharedRO(n1, c1), Unique(n2, c2)) => n2 < n1
-       case (_, Owner) => true
-       case _ => false 
-   }
-   
    
    predicate isWritable(p: Pointer)
    requires valid();
@@ -98,6 +87,16 @@ reads this, tagmem, rawfrom, mem;
       match p.tag
       case Unique(t, c)  => true
       case _ => false
+   }
+   
+   predicate valid_predecessor(tag: Tag, predec: Tag)
+   reads this;
+   {
+     match (tag, predec)
+       case (Unique(n1, c1), Unique(n2, c2)) =>  n2 < n1
+       case (SharedRO(n1, c1), Unique(n2, c2)) => n2 < n1
+       case (_, Owner) => true
+       case _ => false 
    }
    
   method write(p: Pointer, v: int)
@@ -120,11 +119,11 @@ reads this, tagmem, rawfrom, mem;
      
    }
    
+   
    method read(p: Pointer) returns (r: int)
    requires valid();
    // requires p.valid(this);
-   requires valid_addr(p.addr) && p.tag.Unique?;
-   requires p.tag.Unique? ==> p.tag.t <= counter;
+   requires valid_addr(p.addr);
    modifies tagmem;
    ensures forall i :: 0 <= i && i < tagmem.Length && i != p.addr ==> tagmem[i] == old(tagmem[i]);
    ensures forall i :: 0 <= i && i < mem.Length && i != p.addr ==> mem[i] == old(mem[i]);
@@ -141,8 +140,9 @@ reads this, tagmem, rawfrom, mem;
      
      case _ => // ?
    }
-} 
    
+} 
+  
 
    
 
@@ -155,13 +155,15 @@ class Pointer{
  requires s.valid();
  reads s, s.tagmem, s.rawfrom, s.mem, this;
  {
-    s.valid_addr(addr) && valid_predecessor(this.predecessor) &&
-    s.validTag(addr, tag) // && (tag.Unique?  ==> tag.t <= s.counter)
+    s.valid_addr(addr) && s.valid_predecessor(this.tag, this.predecessor) &&
+    s.validTag(addr, tag, predecessor) 
  }
 
-  constructor(addr: nat, tag: Tag, predecessor: Tag, s: State) 
+ 
+ 
+ constructor(addr: nat, tag: Tag, predecessor: Tag, s: State) 
   requires s.valid() && s.valid_addr(addr);
-  requires s.validTag(addr, tag) && s.valid_predecessor(tag, predecessor);
+  requires s.validTag(addr, tag, predecessor) && s.valid_predecessor(tag, predecessor);
   // requires tag.Unique? ==> tag.t == s.counter;
   ensures this.addr == addr && this.tag == tag && /* this.predecessor == predecessor */ s.valid_predecessor(tag, this.predecessor); // under specified
   // ensures this.addr == addr && this.tag == tag && this.predecessor == predecessor;
@@ -193,68 +195,13 @@ ensures s.valid() && ret.valid(s);
        var newtag := Unique(newID, c?);
        s.tagmem[p.addr] := newtag;
        s.rawfrom[p.addr] := -1;
+       assert newID > t;
        ret := new Pointer(p.addr, newtag, p.tag, s);
    // case _ =>
    //    ret := new Pointer(p.addr, Disabled, s);
        // todo
 }
 
-/*
-rawfrom pointers can only be created from Unique(t)
-let raw_pointer = &mut p as *mut i32;
-*/
-method createMutableRawRef(p: Pointer, s: State) returns(ret: Pointer)
-requires s.valid() && s.valid_addr(p.addr);
-requires s.rawfrom[p.addr] == -1 ==> p.tag.Unique?;
-requires s.rawfrom[p.addr] != -1 ==> p.tag.Unique? && s.rawfrom[p.addr] == p.tag.t;
-modifies s, s.tagmem, s.rawfrom;
-ensures s.tagmem == old(s.tagmem) && s.mem == old(s.mem) && s.rawfrom == old(s.rawfrom);
-ensures s.counter == old(s.counter) + 1;
-ensures forall i :: 0 <= i && i < s.tagmem.Length && i != p.addr ==> s.tagmem[i] == old(s.tagmem[i]);
-ensures forall i :: 0 <= i && i < s.rawfrom.Length && i != p.addr ==> s.rawfrom[i] == old(s.rawfrom[i]);
-ensures p.tag.Unique? ==> s.tagmem[p.addr] == ret.tag && s.rawfrom[p.addr] == p.tag.t;
-ensures p.tag.Unique? ==> ret.addr == p.addr && ret.tag == Unique(s.counter, p.tag.c);
-ensures fresh(ret);
-ensures s.valid() && ret.valid(s);
-{
-  var newID := s.generateID();
-  
-  match p.tag
-  case Unique(t, c?) =>
-      var newtag := Unique(newID, c?);
-      s.tagmem[p.addr] := newtag;
-      s.rawfrom[p.addr] := t;
-      ret := new Pointer(p.addr, newtag, s);
-      assert ret.tag.t == s.tagmem[p.addr].t;
-
-}
-
-
-/*
-Rule (NEW-SHARE-REF-1)
-*/
-method createSharedRO(p: Pointer, s: State) returns(ret: Pointer)
-requires s.valid() && s.valid_addr(p.addr);
-requires p.tag.Unique? || p.tag.SharedRO?;
-modifies s, s.tagmem, s.rawfrom;
-ensures s.tagmem == old(s.tagmem) && s.mem == old(s.mem) && s.rawfrom == old(s.rawfrom);
-ensures s.counter == old(s.counter) + 1;
-ensures forall i :: 0 <= i && i < s.tagmem.Length && i != p.addr ==> s.tagmem[i] == old(s.tagmem[i]);
-ensures forall i :: 0 <= i && i < s.rawfrom.Length  ==> s.rawfrom[i] == old(s.rawfrom[i]);
-ensures ret.addr == p.addr && ret.tag == SharedRO(s.counter, p.tag.c);
-ensures fresh(ret);
-ensures s.valid() && ret.valid(s);
-{
-  var newID := s.generateID();
-  var newtag := SharedRO(newID, p.tag.c);
-  match p.tag
-  case Unique(t, c?) =>
-    s.tagmem[p.addr] := newtag;
-    ret := new Pointer(p.addr, newtag, s);
-  case SharedRO(t, c?) =>
-    s.tagmem[p.addr] := newtag;
-    ret := new Pointer(p.addr, newtag, s);
-}
 
 // This client follows stack principle
 // C1
@@ -313,54 +260,4 @@ method mutableTest2(mem:array<int>)
     assert !ref3.valid(s);
   }
   
-}
-
-
-method mutableRawTest(mem:array<int>)
-  modifies mem;
-{
-    var s := new State(mem);
-        
-    // let mut local1 = 5;
-    var local1: nat;
-    var tag1 := s.generateID();
-    if(0 < local1 < mem.Length){
-      mem[local1] := 5;
-      var ref1: Pointer := new Pointer(local1, Unique(tag1, 1), s);
-     // s.write(ref1, 42);
-      var ref2: Pointer := createMutableRawRef(ref1, s);
-      assert(ref2.valid(s));
-
-      var ref3: Pointer := createMutableRawRef(ref1, s);
-      assert(!ref2.valid(s));
-
-      var ref4: Pointer := createMutableRawRef(ref1, s);
-      assert(!ref3.valid(s));
-    }
-
-  }
-
-method mutableSharedROTest(mem:array<int>)
-modifies mem;
-{
-  var s := new State(mem);
-        
-  // let mut local1 = 5;
-  var local1: nat;
-  var tag1 := s.generateID();
-  if(0 < local1 < mem.Length){
-      mem[local1] := 5;
-      var ref1: Pointer := new Pointer(local1, Unique(tag1, 1), s);
-     // s.write(ref1, 42);
-      var ref2: Pointer := createMutableRef(ref1, s);
-      
-      assert(ref2.valid(s));
-      var ref3: Pointer := createSharedRO(ref2, s);
-      assert(ref3.valid(s));
-      var ref4: Pointer := createSharedRO(ref2, s);
-      assert(ref4.valid(s));
-      var ref5: Pointer := createMutableRef(ref2, s);
-      assert(!ref4.valid(s));
-
-  }
 }
